generalize induction helpers

Alg/ListProps/Sorted/Induction.lean
@@ -10,7 +10,7 @@ def List.sorted.induction.bounded
   [Compare α] 
   {P: List α -> List α -> Sort _}
   (empty_left: ∀bs, P [] bs)
-  (empty_right: ∀as, P as [])
+  (empty_right: ∀a as, P (a::as) [])
   (induct_lt: ∀a as b bs, Compare.ord a b = Order.Less -> P as (b::bs) -> P (a::as) (b::bs))
   (induct_eq: ∀a as b bs, Compare.ord a b = Order.Eq -> P as bs -> P (a::as) (b::bs))
   (induct_gt: ∀a as b bs, Compare.ord a b = Order.Greater -> P (a::as) bs -> P (a::as) (b::bs))
@@ -38,7 +38,7 @@ def List.sorted.induction.bounded
   match as with
   | [] => exact empty_left bs
   | a::as' => match bs with
-    | [] => exact empty_right (a::as')
+    | [] => exact empty_right a as'
     | b::bs' => match h:Compare.ord a b with
       | .Less => 
       have := List.sorted.induction.bounded
@@ -82,7 +82,7 @@ theorem List.sorted.induction.bounded.fuel_irr
   [Compare α] 
   {P: List α -> List α -> Sort _}
   (empty_left: ∀bs, P [] bs)
-  (empty_right: ∀as, P as [])
+  (empty_right: ∀a as, P (a::as) [])
   (induct_lt: ∀a as b bs, Compare.ord a b = Order.Less -> P as (b::bs) -> P (a::as) (b::bs))
   (induct_eq: ∀a as b bs, Compare.ord a b = Order.Eq -> P as bs -> P (a::as) (b::bs))
   (induct_gt: ∀a as b bs, Compare.ord a b = Order.Greater -> P (a::as) bs -> P (a::as) (b::bs))
@@ -147,7 +147,7 @@ def List.sorted.induction
   [Compare α] 
   {P: List α -> List α -> Sort _}
   (empty_left: ∀bs, P [] bs)
-  (empty_right: ∀as, P as [])
+  (empty_right: ∀a as, P (a::as) [])
   (induct_lt: ∀a as b bs, Compare.ord a b = Order.Less -> P as (b::bs) -> P (a::as) (b::bs))
   (induct_eq: ∀a as b bs, Compare.ord a b = Order.Eq -> P as bs -> P (a::as) (b::bs))
   (induct_gt: ∀a as b bs, Compare.ord a b = Order.Greater -> P (a::as) bs -> P (a::as) (b::bs))
@@ -162,7 +162,7 @@ theorem List.sorted.induction.unfuel
   [Compare α] 
   {P: List α -> List α -> Sort _}
   (empty_left: ∀bs, P [] bs)
-  (empty_right: ∀as, P as [])
+  (empty_right: ∀a as, P (a::as) [])
   (induct_lt: ∀a as b bs, Compare.ord a b = Order.Less -> P as (b::bs) -> P (a::as) (b::bs))
   (induct_eq: ∀a as b bs, Compare.ord a b = Order.Eq -> P as bs -> P (a::as) (b::bs))
   (induct_gt: ∀a as b bs, Compare.ord a b = Order.Greater -> P (a::as) bs -> P (a::as) (b::bs))
@@ -177,3 +177,353 @@ theorem List.sorted.induction.unfuel
   rw [List.sorted.induction.bounded.fuel_irr]
 
 #print axioms List.sorted.induction.unfuel
+
+theorem List.sorted.empty_left.helper [Compare α]
+  {P: List α -> List α -> Sort _}
+  (empty_left: ∀bs, P [] bs)
+  (empty_right: ∀a as, P (a::as) [])
+  (induct_lt: ∀a as b bs, Compare.ord a b = Order.Less -> P as (b::bs) -> P (a::as) (b::bs))
+  (induct_eq: ∀a as b bs, Compare.ord a b = Order.Eq -> P as bs -> P (a::as) (b::bs))
+  (induct_gt: ∀a as b bs, Compare.ord a b = Order.Greater -> P (a::as) bs -> P (a::as) (b::bs))
+: ∀{as bs: List α}, as = [] -> List.sorted.induction empty_left empty_right induct_lt induct_eq induct_gt [] bs = empty_left bs
+ := by
+  apply List.sorted.induction
+
+  {
+    intro bs
+    intro _
+    match bs with
+    | [] => rfl
+    | b::bs' => rfl
+  }
+
+  {
+    intro a _
+    intro as_is_empty
+    contradiction
+  }
+
+  repeat {
+    intro _ _ _ _ _ _ _
+    contradiction
+  }
+
+#print axioms List.sorted.empty_left.helper
+
+theorem List.sorted.empty_left [Compare α]
+  {P: List α -> List α -> Sort _}
+  (empty_left: ∀bs, P [] bs)
+  (empty_right: ∀a as, P (a::as) [])
+  (induct_lt: ∀a as b bs, Compare.ord a b = Order.Less -> P as (b::bs) -> P (a::as) (b::bs))
+  (induct_eq: ∀a as b bs, Compare.ord a b = Order.Eq -> P as bs -> P (a::as) (b::bs))
+  (induct_gt: ∀a as b bs, Compare.ord a b = Order.Greater -> P (a::as) bs -> P (a::as) (b::bs)) :
+  ∀(bs: List α),
+   List.sorted.induction empty_left empty_right induct_lt induct_eq induct_gt [] bs = empty_left bs := by
+  intro bs
+  apply List.sorted.empty_left.helper
+  rfl
+
+#print axioms List.sorted.empty_left
+
+theorem List.sorted.empty_right.helper [Compare α]
+  {P: List α -> List α -> Sort _}
+  (empty_left: ∀bs, P [] bs)
+  (empty_right: ∀a as, P (a::as) [])
+  (induct_lt: ∀a as b bs, Compare.ord a b = Order.Less -> P as (b::bs) -> P (a::as) (b::bs))
+  (induct_eq: ∀a as b bs, Compare.ord a b = Order.Eq -> P as bs -> P (a::as) (b::bs))
+  (induct_gt: ∀a as b bs, Compare.ord a b = Order.Greater -> P (a::as) bs -> P (a::as) (b::bs))
+: ∀{as bs: List α}, ∀x xs, as = x::xs -> bs = [] -> List.sorted.induction empty_left empty_right induct_lt induct_eq induct_gt (x::xs) [] = empty_right x xs
+ := by
+  apply List.sorted.induction
+
+
+  {
+    intro _
+    intro x xs a_eq_xs _
+    contradiction
+  }
+
+  {
+    intro a as
+    intro x xs _ _
+    rfl
+  }
+
+  repeat {
+    intro _ _ _ _ _ _
+    intro x xs a_eq_xs b_eq_empty
+    contradiction
+  }
+
+#print axioms List.sorted.empty_right.helper
+
+theorem List.sorted.empty_right [Compare α]
+  {P: List α -> List α -> Sort _}
+  (empty_left: ∀bs, P [] bs)
+  (empty_right: ∀a as, P (a::as) [])
+  (induct_lt: ∀a as b bs, Compare.ord a b = Order.Less -> P as (b::bs) -> P (a::as) (b::bs))
+  (induct_eq: ∀a as b bs, Compare.ord a b = Order.Eq -> P as bs -> P (a::as) (b::bs))
+  (induct_gt: ∀a as b bs, Compare.ord a b = Order.Greater -> P (a::as) bs -> P (a::as) (b::bs)) :
+  ∀(a: α) (as: List α),
+   List.sorted.induction empty_left empty_right induct_lt induct_eq induct_gt (a::as) [] = empty_right a as := by
+  intro a as
+  apply List.sorted.empty_right.helper
+  rfl
+  rfl
+
+theorem List.sorted.induct_lt.helper [Compare α]
+  {P: List α -> List α -> Sort _}
+  (empty_left: ∀bs, P [] bs)
+  (empty_right: ∀a as, P (a::as) [])
+  (induct_lt: ∀a as b bs, Compare.ord a b = Order.Less -> P as (b::bs) -> P (a::as) (b::bs))
+  (induct_eq: ∀a as b bs, Compare.ord a b = Order.Eq -> P as bs -> P (a::as) (b::bs))
+  (induct_gt: ∀a as b bs, Compare.ord a b = Order.Greater -> P (a::as) bs -> P (a::as) (b::bs)) :
+  ∀(as bs cs ds: List α) (c d: α) (fuel fuel_def), as = c::cs -> bs = d::ds -> (c_ord_d: Compare.ord c d = Order.Less) -> List.sorted.induction empty_left empty_right induct_lt induct_eq induct_gt (c::cs) (d::ds) = induct_lt c cs d ds c_ord_d (
+    induction.bounded empty_left empty_right induct_lt induct_eq induct_gt cs (d :: ds) fuel fuel_def
+  ) := by
+  apply List.sorted.induction
+
+  {
+    intro bs
+    intro cs ds c d as_eq_cs _ _
+    contradiction
+  }
+
+  {
+    intro a as
+    intro cs ds c d fuel fuel_def _ bs_eq_ds c_ord_d
+    contradiction
+  }
+
+  {
+    intro a as b bs a_ord_b _
+    intro cs ds c d fuel fuel_def as_eq_cs bs_eq_ds c_ord_d
+    have ⟨ a_eq_c, as_eq_cs ⟩  := List.cons.inj as_eq_cs
+    have ⟨ b_eq_d, bs_eq_ds ⟩  := List.cons.inj bs_eq_ds
+    conv => {
+      lhs
+      unfold sorted sorted.induction sorted.induction.bounded
+    }
+    simp
+    split
+    contradiction
+    contradiction
+    split
+    rw [induction.bounded.fuel_irr]
+    rw [c_ord_d] at *
+    contradiction
+    rw [c_ord_d] at *
+    contradiction
+  }
+
+  {
+    intro a as b bs a_ord_b _
+    intro cs ds c d fuel fuel_def as_eq_cs bs_eq_ds c_ord_d
+    have ⟨ a_eq_c, as_eq_cs ⟩  := List.cons.inj as_eq_cs
+    have ⟨ b_eq_d, bs_eq_ds ⟩  := List.cons.inj bs_eq_ds
+    rw [a_eq_c, b_eq_d] at a_ord_b
+    rw [a_ord_b] at c_ord_d
+    contradiction
+  }
+
+  {
+    intro a as b bs a_ord_b _
+    intro cs ds c d fuel fuel_def as_eq_cs bs_eq_ds c_ord_d
+    have ⟨ a_eq_c, as_eq_cs ⟩  := List.cons.inj as_eq_cs
+    have ⟨ b_eq_d, bs_eq_ds ⟩  := List.cons.inj bs_eq_ds
+    rw [a_eq_c, b_eq_d] at a_ord_b
+    rw [a_ord_b] at c_ord_d
+    contradiction
+  }
+
+#print axioms List.sorted.induct_lt.helper
+
+theorem List.sorted.induct_lt [Compare α]
+  {P: List α -> List α -> Sort _}
+  (empty_left: ∀bs, P [] bs)
+  (empty_right: ∀a as, P (a::as) [])
+  (induct_lt: ∀a as b bs, Compare.ord a b = Order.Less -> P as (b::bs) -> P (a::as) (b::bs))
+  (induct_eq: ∀a as b bs, Compare.ord a b = Order.Eq -> P as bs -> P (a::as) (b::bs))
+  (induct_gt: ∀a as b bs, Compare.ord a b = Order.Greater -> P (a::as) bs -> P (a::as) (b::bs)) :
+  ∀(a b: α) (as bs: List α) (a_ord_b: Compare.ord a b = Order.Less),
+   List.sorted.induction empty_left empty_right induct_lt induct_eq induct_gt (a::as) (b::bs) = induct_lt a as b bs a_ord_b (
+    induction empty_left empty_right induct_lt induct_eq induct_gt as (b :: bs)
+  ) := by
+  intro a b as bs a_ord_b
+  apply List.sorted.induct_lt.helper
+  rfl
+  rfl
+
+#print axioms List.sorted.induct_lt
+
+theorem List.sorted.induct_eq.helper [Compare α]
+  {P: List α -> List α -> Sort _}
+  (empty_left: ∀bs, P [] bs)
+  (empty_right: ∀a as, P (a::as) [])
+  (induct_lt: ∀a as b bs, Compare.ord a b = Order.Less -> P as (b::bs) -> P (a::as) (b::bs))
+  (induct_eq: ∀a as b bs, Compare.ord a b = Order.Eq -> P as bs -> P (a::as) (b::bs))
+  (induct_gt: ∀a as b bs, Compare.ord a b = Order.Greater -> P (a::as) bs -> P (a::as) (b::bs)) :
+  ∀(as bs cs ds: List α) (c d: α) (fuel fuel_def), as = c::cs -> bs = d::ds -> (c_ord_d: Compare.ord c d = Order.Eq) -> List.sorted.induction empty_left empty_right induct_lt induct_eq induct_gt (c::cs) (d::ds) = induct_eq c cs d ds c_ord_d (
+    induction.bounded empty_left empty_right induct_lt induct_eq induct_gt cs ds fuel fuel_def
+  ) := by
+  apply List.sorted.induction
+
+  {
+    intro bs
+    intro cs ds c d as_eq_cs _ _
+    contradiction
+  }
+
+  {
+    intro a as
+    intro cs ds c d fuel fuel_def _ bs_eq_ds c_ord_d
+    contradiction
+  }
+
+  {
+    intro a as b bs a_ord_b _
+    intro cs ds c d fuel fuel_def as_eq_cs bs_eq_ds c_ord_d
+    have ⟨ a_eq_c, as_eq_cs ⟩  := List.cons.inj as_eq_cs
+    have ⟨ b_eq_d, bs_eq_ds ⟩  := List.cons.inj bs_eq_ds
+    rw [a_eq_c, b_eq_d] at a_ord_b
+    rw [a_ord_b] at c_ord_d
+    contradiction
+  }
+
+  {
+    intro a as b bs a_ord_b _
+    intro cs ds c d fuel fuel_def as_eq_cs bs_eq_ds c_ord_d
+    
+    have ⟨ a_eq_c, as_eq_cs ⟩  := List.cons.inj as_eq_cs
+    have ⟨ b_eq_d, bs_eq_ds ⟩  := List.cons.inj bs_eq_ds
+    conv => {
+      lhs
+      unfold sorted sorted.induction sorted.induction.bounded
+    }
+    simp
+    split
+    contradiction
+    contradiction
+    split
+    rw [c_ord_d] at *
+    contradiction
+    rw [induction.bounded.fuel_irr]
+    rw [c_ord_d] at *
+    contradiction
+  }
+
+  {
+    intro a as b bs a_ord_b _
+    intro cs ds c d fuel fuel_def as_eq_cs bs_eq_ds c_ord_d
+    have ⟨ a_eq_c, as_eq_cs ⟩  := List.cons.inj as_eq_cs
+    have ⟨ b_eq_d, bs_eq_ds ⟩  := List.cons.inj bs_eq_ds
+    rw [a_eq_c, b_eq_d] at a_ord_b
+    rw [a_ord_b] at c_ord_d
+    contradiction
+  }
+
+#print axioms List.sorted.induct_eq.helper
+
+theorem List.sorted.induct_eq [Compare α]
+  {P: List α -> List α -> Sort _}
+  (empty_left: ∀bs, P [] bs)
+  (empty_right: ∀a as, P (a::as) [])
+  (induct_lt: ∀a as b bs, Compare.ord a b = Order.Less -> P as (b::bs) -> P (a::as) (b::bs))
+  (induct_eq: ∀a as b bs, Compare.ord a b = Order.Eq -> P as bs -> P (a::as) (b::bs))
+  (induct_gt: ∀a as b bs, Compare.ord a b = Order.Greater -> P (a::as) bs -> P (a::as) (b::bs)) :
+  ∀(a b: α) (as bs: List α) (a_ord_b: Compare.ord a b = Order.Eq),
+   List.sorted.induction empty_left empty_right induct_lt induct_eq induct_gt (a::as) (b::bs) = induct_eq a as b bs a_ord_b (
+    induction empty_left empty_right induct_lt induct_eq induct_gt as bs
+  ) := by
+  intro a b as bs a_ord_b
+  apply List.sorted.induct_eq.helper
+  rfl
+  rfl
+
+#print axioms List.sorted.induct_eq
+
+theorem List.sorted.induct_gt.helper [Compare α]
+  {P: List α -> List α -> Sort _}
+  (empty_left: ∀bs, P [] bs)
+  (empty_right: ∀a as, P (a::as) [])
+  (induct_lt: ∀a as b bs, Compare.ord a b = Order.Less -> P as (b::bs) -> P (a::as) (b::bs))
+  (induct_eq: ∀a as b bs, Compare.ord a b = Order.Eq -> P as bs -> P (a::as) (b::bs))
+  (induct_gt: ∀a as b bs, Compare.ord a b = Order.Greater -> P (a::as) bs -> P (a::as) (b::bs)) :
+  ∀(as bs cs ds: List α) (c d: α) (fuel fuel_def), as = c::cs -> bs = d::ds -> (c_ord_d: Compare.ord c d = Order.Greater) -> List.sorted.induction empty_left empty_right induct_lt induct_eq induct_gt (c::cs) (d::ds) = induct_gt c cs d ds c_ord_d (
+    induction.bounded empty_left empty_right induct_lt induct_eq induct_gt (c::cs) ds fuel fuel_def
+  ) := by
+  apply List.sorted.induction
+
+  {
+    intro bs
+    intro cs ds c d as_eq_cs _ _
+    contradiction
+  }
+
+  {
+    intro a as
+    intro cs ds c d fuel fuel_def _ bs_eq_ds c_ord_d
+    contradiction
+  }
+
+  {
+    intro a as b bs a_ord_b _
+    intro cs ds c d fuel fuel_def as_eq_cs bs_eq_ds c_ord_d
+    have ⟨ a_eq_c, as_eq_cs ⟩  := List.cons.inj as_eq_cs
+    have ⟨ b_eq_d, bs_eq_ds ⟩  := List.cons.inj bs_eq_ds
+    rw [a_eq_c, b_eq_d] at a_ord_b
+    rw [a_ord_b] at c_ord_d
+    contradiction
+  }
+
+  {
+    intro a as b bs a_ord_b _
+    intro cs ds c d fuel fuel_def as_eq_cs bs_eq_ds c_ord_d
+    have ⟨ a_eq_c, as_eq_cs ⟩  := List.cons.inj as_eq_cs
+    have ⟨ b_eq_d, bs_eq_ds ⟩  := List.cons.inj bs_eq_ds
+    rw [a_eq_c, b_eq_d] at a_ord_b
+    rw [a_ord_b] at c_ord_d
+    contradiction
+  }
+
+  {
+    intro a as b bs a_ord_b _
+    intro cs ds c d fuel fuel_def as_eq_cs bs_eq_ds c_ord_d
+    
+    have ⟨ a_eq_c, as_eq_cs ⟩  := List.cons.inj as_eq_cs
+    have ⟨ b_eq_d, bs_eq_ds ⟩  := List.cons.inj bs_eq_ds
+    conv => {
+      lhs
+      unfold sorted sorted.induction sorted.induction.bounded
+    }
+    simp
+    split
+    contradiction
+    contradiction
+    split
+    rw [c_ord_d] at *
+    contradiction
+    rw [c_ord_d] at *
+    contradiction
+    rw [induction.bounded.fuel_irr]
+  }
+
+#print axioms List.sorted.induct_eq.helper
+
+theorem List.sorted.induct_gt [Compare α]
+  {P: List α -> List α -> Sort _}
+  (empty_left: ∀bs, P [] bs)
+  (empty_right: ∀a as, P (a::as) [])
+  (induct_lt: ∀a as b bs, Compare.ord a b = Order.Less -> P as (b::bs) -> P (a::as) (b::bs))
+  (induct_eq: ∀a as b bs, Compare.ord a b = Order.Eq -> P as bs -> P (a::as) (b::bs))
+  (induct_gt: ∀a as b bs, Compare.ord a b = Order.Greater -> P (a::as) bs -> P (a::as) (b::bs)) :
+  ∀(a b: α) (as bs: List α) (a_ord_b: Compare.ord a b = Order.Greater),
+   List.sorted.induction empty_left empty_right induct_lt induct_eq induct_gt (a::as) (b::bs) = induct_gt a as b bs a_ord_b (
+    induction empty_left empty_right induct_lt induct_eq induct_gt (a::as) bs
+  ) := by
+  intro a b as bs a_ord_b
+  apply List.sorted.induct_gt.helper
+  rfl
+  rfl
+
+#print axioms List.sorted.induct_eq
